updates

theories/Examples/ConcurrentHashTable.v
@@ -9,27 +9,29 @@
    - Std: [Crane Extract Inlined Constant CHT.max => "std::max(%a0, %a1)".]
    - BDE: [Crane Extract Inlined Constant CHT.max => "bsl::max(%a0, %a1)".]
 *)
-From Stdlib Require Import List Bool Vector.
+From Stdlib Require Import List Bool Nat.
 From Crane Require Extraction.
-From Crane Require Import Monads.ITree Monads.IODefs Monads.STMDefs External.VectorDefs.
-From Corelib Require Import PrimInt63.
+From Crane Require Import Monads.ITree Monads.IODefs Monads.STMDefs.
 
 Import ListNotations.
 Set Implicit Arguments.
 
+(*
 Axiom nat_of_int : int -> nat.
 Crane Extract Inlined Constant nat_of_int => "static_cast<unsigned int>(%a0)".
+*)
+
+From ITree Require Import Eq Props.HasPost.
+From Paco Require Import paco.
 
 Module CHT.
-
-Open Scope int63.
 
 Section key_val.
 
 Context {K V : Type}.
 
 Definition const_type : unit -> Type :=
-  fun _ => V.
+  fun _ => list (K * V).
 
 #[local] Notation TVar := (TVar const_type).
 #[local] Notation stmE := (stmE const_type).
@@ -66,37 +68,38 @@ Fixpoint assoc_remove
 
 Record CHT := {
   cht_eqb     : K -> K -> bool;
-  cht_hash    : K -> int;
+  cht_hash    : K -> nat;
   cht_nbuckets: nat;
-  cht_buckets : Vector.t (TVar (list (K * V))) cht_nbuckets;
-  cht_fallback: TVar (list (K * V))           (* first bucket as a total fallback *)
+  cht_buckets : list (TVar (list (K * V)));
+  cht_fallback : TVar (list (K * V));
+  cht_buckets_wf : length cht_buckets = cht_nbuckets
 }.
 
 (* Total bucket selection *)
 Definition bucket_of (t : CHT) (k : K)
-  :  itree stmE (TVar (list (K * V))) :=
-  let i := mod (t.(cht_hash) k) t.(cht_nbuckets) in
-  t.(cht_buckets) i.
+  :  TVar (list (K * V)) :=
+  let i := modulo (t.(cht_hash) k) t.(cht_nbuckets) in
+  nth i t.(cht_buckets) t.(cht_fallback).
 
 Section STM.
 
 (* Get *)
-Definition stm_get {K V} (t : CHT K V) (k : K) : itree stmE (option V) :=
-  b <- bucket_of t k ;;
+Definition stm_get (t : CHT) (k : K) : itree stmE (option V) :=
+  let b := bucket_of t k in
   xs <- readTVar b ;;
   Ret (assoc_lookup t.(cht_eqb) k xs).
 
 (* Put / upsert *)
-Definition stm_put {K V} (t : CHT K V) (k : K) (v : V) : itree stmE unit :=
-  b <- bucket_of t k ;;
+Definition stm_put (t : CHT) (k : K) (v : V) : itree stmE unit :=
+  let b := bucket_of t k in
   xs <- readTVar b ;;
   let xs' := assoc_insert_or_replace t.(cht_eqb) k v xs in
   writeTVar b xs' ;;
   Ret tt.
 
 (* Delete; returns previous value if any *)
-Definition stm_delete {K V} (t : CHT K V) (k : K) : itree stmE (option V) :=
-  b <- bucket_of t k ;;
+Definition stm_delete (t : CHT) (k : K) : itree stmE (option V) :=
+  let b := bucket_of t k in
   xs <- readTVar b ;;
   let p := assoc_remove t.(cht_eqb) k xs in
   match fst p with
@@ -107,9 +110,9 @@ Definition stm_delete {K V} (t : CHT K V) (k : K) : itree stmE (option V) :=
   end.
 
 (* Update with a function of the old option; returns the new value *)
-Definition stm_update {K V}
-           (t : CHT K V) (k : K) (f : option V -> V) : itree stmE V :=
-  b <- bucket_of t k ;;
+Definition stm_update
+           (t : CHT) (k : K) (f : option V -> V) : itree stmE V :=
+  let b := bucket_of t k in
   xs <- readTVar b ;;
   let ov := assoc_lookup t.(cht_eqb) k xs in
   let v  := f ov in
@@ -117,49 +120,148 @@ Definition stm_update {K V}
   writeTVar b xs' ;;
   Ret v.
 
-Definition stm_get_or {K V} (t : CHT K V) (k : K) (dflt : V) : itree stmE V :=
+Definition stm_get_or (t : CHT) (k : K) (dflt : V) : itree stmE V :=
   v <- stm_get t k ;;
   match v with
   | Some x => Ret x
   | None => Ret dflt
   end.
 
+(*
 Definition max : int -> int -> int := fun a b =>
   if ltb a b then b else a.
+*)
 
 End STM.
 
-Definition vecIOE := vectorE +' ioE.
-Crane Extract Skip vecIOE.
+#[local] Notation runStmE := (runStmE const_type).
+
+Definition runStmIOE := runStmE +' ioE.
 
 (* Build N empty buckets *)
-Definition mk_buckets {K V} (num : int) : itree vecIOE (vector (TVar (list (K * V)))) :=
-  buckets <- (emptyVec (TVar (list (K * V)))) ;;
-  (fix f n := match n with
-  | 0 => Ret buckets
-  | S n' =>
-    b <- atomically (newTVar ([] : list (K * V))) ;;
-    push buckets b ;;
-    f n'
-  end) (nat_of_int num).
+Definition mk_buckets (num : nat) : itree runStmIOE (list (TVar (list (K * V)))) :=
+  (fix f buckets n :=
+    match n with
+    | 0 => Ret buckets
+    | S n' =>
+        b <- atomically (newTVar tt []) ;;
+        f (b :: buckets) n'
+    end) [] num.
+
+Lemma has_post_subrel : forall {E R} (t : itree E R) (P Q : R -> Prop),
+  (forall x, P x -> Q x) ->
+  has_post t P ->
+  has_post t Q.
+Proof.
+  intros.
+  eapply eutt_subrel, H0.
+  intros ??.
+  apply H.
+Qed.
+
+Lemma mk_buckets_length : forall n, has_post (mk_buckets n) (fun buckets => length buckets = n).
+Proof.
+  intros.
+  unfold mk_buckets.
+  apply has_post_subrel with (P := fun buckets => length buckets = n + length ([] : list (TVar (const_type tt)))).
+  { intros. rewrite plus_n_O. apply H. }
+  generalize ([] : list (TVar (const_type tt))).
+  induction n.
+  - intros. apply eutt_Ret. reflexivity.
+  - intros.
+    apply has_post_bind_weak.
+    intros.
+    cbn. rewrite plus_n_Sm.
+    apply IHn.
+Qed.
+
+
+
+Lemma has_post_eta {E R} {P : R -> Prop} (t : itree E R) : has_post t P -> has_post (go (observe t)) P.
+Proof.
+  intros.
+  rewrite <- itree_eta.
+  assumption.
+Qed.
+
+Lemma has_post_inv_Ret {E R} {P : R -> Prop} (r : R) : has_post ((Ret r) : itree E R) P -> P r.
+Proof.
+  intros.
+  apply eqit_inv_Ret in H.
+  apply H.
+Qed.
+
+Lemma has_post_inv_Tau {E R} {P : R -> Prop} (t : itree E R) : has_post (Tau t) P -> has_post t P.
+Proof.
+  intros.
+  apply eqit_inv_Tau in H.
+  apply H.
+Qed.
+
+Lemma has_post_inv_Vis {E R} {P : R -> Prop} {X} (e : E X) (k : X -> itree E R) : has_post (Vis e k) P -> forall x, has_post (k x) P.
+Proof.
+  intros.
+  eapply eqit_inv_Vis in H.
+  apply H.
+Qed.
+
+CoFixpoint with_post {E R} {P : R -> Prop} (t : itree E R) (pf : has_post t P) : itree E {x:R | P x} :=
+  let ot := observe t in
+  let pf' := has_post_eta pf in
+  (match ot return ot = observe t -> _ with
+  | RetF r => fun Heqot => Ret (exist P r (has_post_inv_Ret (eq_ind_r (fun ot => has_post (go ot) P) pf' Heqot)))
+  | TauF t => fun Heqot => Tau (@with_post E R P t (has_post_inv_Tau (eq_ind_r (fun ot => has_post (go ot) P) pf' Heqot)))
+  | VisF e k => fun Heqot => Vis e (fun x => @with_post E R P (k x) (has_post_inv_Vis (eq_ind_r (fun ot => has_post (go ot) P) pf' Heqot) x))
+  end) eq_refl.
+
+Arguments with_post : clear implicits.
+Arguments with_post {E R P} (t pf).
+
+Notation with_post_ P t pf :=
+  (let ot := observe t in
+  let pf' := has_post_eta pf in
+  (match ot return ot = observe t -> _ with
+  | RetF r => fun Heqot => Ret (exist P r (has_post_inv_Ret (eq_ind_r (fun ot => has_post (go ot) P) pf' Heqot)))
+  | TauF t => fun Heqot => Tau (@with_post _ _ P t (has_post_inv_Tau (eq_ind_r (fun ot => has_post (go ot) P) pf' Heqot)))
+  | VisF e k => fun Heqot => Vis e (fun x => @with_post _ _ P (k x) (has_post_inv_Vis (eq_ind_r (fun ot => has_post (go ot) P) pf' Heqot) x))
+  end) eq_refl).
+
+
+
+Lemma unfold_with_post {E R} (P : R -> Prop) (t : itree E R) (pf : has_post t P) :
+  with_post t pf ≅ with_post_ P t pf.
+Proof.
+  apply observing_sub_eqit; constructor; reflexivity.
+Qed.
+
+
+Lemma with_post_proj1 {E R} {P : R -> Prop} (t : itree E R) (pf : has_post t P) :
+  ITree.map (@proj1_sig R P) (with_post t pf) ≅ t.
+Proof.
+  revert t pf.
+  unfold ITree.map.
+  ginit.
+  gcofix CIH.
+  intros.
+  rewrite unfold_with_post.
+  gstep.
+  generalize (observe t).
+  red in pf.
+Abort.
+
 
 (* Create a new table with at least one bucket; stores eqb/hash in the record *)
-Definition new_hash {K V}
-           (eqb : K -> K -> bool) (hash : K -> int) (requested : int)
-  : itree vecIOE (CHT K V) :=
+Definition new_hash
+           (eqb : K -> K -> bool) (hash : K -> nat) (requested : nat)
+  : itree runStmIOE CHT :=
   let n := max requested 1 in
-  bs <- mk_buckets (K:=K) (V:=V) n ;;
-  empt <- isEmpty bs ;;
-  if empt then
-      fb <- atomically (newTVar ([] : list (K * V))) ;;
-      v <- emptyVec (TVar (list (K * V))) ;;
-      push v fb ;;
-      Ret {| cht_eqb := eqb; cht_hash := hash;
-                cht_buckets := v; cht_nbuckets := 1; cht_fallback := fb |}
-  else
-    b <- get bs 0 ;;
-    Ret {| cht_eqb := eqb; cht_hash := hash;
-                cht_buckets := bs; cht_nbuckets := n; cht_fallback := b |}.
+  '(exist _ buckets Hbuckets) <- with_post (mk_buckets n) (mk_buckets_length n) ;;
+  _.
+(*
+  fallback <- get bs 0 ;;
+  Ret {| cht_eqb := eqb; cht_hash := hash;
+         cht_buckets := bs; cht_nbuckets := n; cht_fallback := b |}.
+*)
 
 Definition put  {K V} (t : CHT K V) (k : K) (v : V) : itree ioE unit :=
   atomically (stm_put t k v).
