theories/Monads/STMDefs2.v
@@ -1,0 +1,212 @@
+(* Copyright 2025 Bloomberg Finance L.P. *)
+(* Distributed under the terms of the GNU LGPL v2.1 license. *)
+(**
+   Shared STM effect definitions (flavor-independent).
+
+   Contains the effect inductives ([tvarE], [stmVecE], [stmControlE]),
+   composed effect ([stmE]), axioms, and smart constructors that are
+   identical across library flavors. Flavor files ([STM.v], [STMBDE.v])
+   re-export this module and add flavor-specific C++ extraction mappings.
+*)
+From Corelib Require Import PrimString.
+From Crane Require Extraction.
+From Crane Require Import Monads.ITree.
+
+From ITree Require Import Basics.Basics.
+
+Open Scope itree_scope.
+
+Axiom TVar : Type -> Type.
+
+Inductive tvarE : Type -> Type :=
+| NewTVar : forall {A}, A -> tvarE (TVar A)
+| ReadTVar : forall {A}, TVar A -> tvarE A
+| WriteTVar : forall {A}, TVar A -> A -> tvarE unit.
+
+
+Inductive stmControlE : Type -> Type :=
+| Retry : stmControlE void.
+
+Crane Extract Inductive stmControlE => ""
+  [ "stm::retry()" ].
+
+Definition stmE : Type -> Type := stmControlE +' tvarE.
+Crane Extract Skip stmE.
+
+Definition retry {A} : itree stmE A :=
+  trigger (inl1 Retry) >>= fun (x : void) => match x with end.
+
+(* not entirely sure why this is required *)
+(*
+#[global] Instance tvarE_sub_stmE {K} (V : K -> Type) : tvarE V -< stmE V := inr1.
+#[global] Instance stmControlE_sub_stmE {K} (V : K -> Type) : stmControlE -< stmE V := inl1.
+Crane Extract Skip tvarE_sub_stmE.
+Crane Extract Skip stmControlE_sub_stmE.
+*)
+
+
+
+Variant runStmE : Type -> Type :=
+| Atomically : forall {A} (t : itree stmE A), runStmE A.
+
+Definition atomically {E} `{runStmE -< E} {A} (t : itree stmE A) : itree E A :=
+  trigger (Atomically t).
+
+Crane Extract Inductive runStmE => ""
+  [ "stm::atomically([&] { return %a0; })" ].
+
+
+
+(*
+Definition orElse {A} {K} {V : K -> Type} `{EqDec K eq} (t1 t2 : itree (stmControlE +' tvarE V) A) : itree (stmE V) A :=
+  (cofix _orElse (m : halist (pkey K nat) (pkey_type V)) t :=
+    match observe t with
+    | RetF a =>
+        commit_log V m ;;
+        Ret a
+    | TauF t => Tau (_orElse m t)
+    | VisF (inr1 e) k => '(x, m) <- handle_tvar_log m e ;; Tau (_orElse m (k x))
+    | VisF (inl1 Retry) _ => t2
+    end) HMap.empty t1.
+*)
+
+
+
+Definition newTVar {A} (a : A) : itree stmE (TVar A) := trigger (inr1 (NewTVar a)).
+Definition readTVar {A} (v : TVar A) : itree stmE A := trigger (inr1 (ReadTVar v)).
+Definition writeTVar {A} (v : TVar A) (a : A) : itree stmE unit := trigger (inr1 (WriteTVar v a)).
+
+Definition check (b : bool) : itree stmE unit :=
+  if b then Ret tt else retry.
+
+Definition modifyTVar {A} (a : TVar A) (f : A -> A) : itree stmE unit :=
+  val <- readTVar a ;;
+  writeTVar a (f val) ;;
+  Ret tt.
+
+Crane Extract Inlined Constant atomically => "stm::atomically([&] { return %a0; })".
+(*Crane Extract Inlined Constant orElse => "stm::orElse<%t0>(%a0, %a1)".*)
+Crane Extract Inlined Constant retry => "stm::retry<%t2>()".
+Crane Extract Inlined Constant newTVar => "stm::newTVar(%a1)".
+
+
+
+From ITree Require Import Basics.Basics.
+
+Import Basics.Monads.
+
+Variant h_tvarE_spec : forall A, tvarE A -> (TVar ~> option) -> A -> (TVar ~> option) -> Prop :=
+| h_NewTVar {A} (a : A) (x : TVar A) s1 s2 :
+    s1 _ x = None ->
+    s2 _ x = Some a ->
+    (* s2 is the same as s1 except for x *) True ->
+    h_tvarE_spec (TVar A) (NewTVar a) s1 x s2
+| h_ReadTVar {A} (x : TVar A) (a : A) s :
+    s _ x = Some a ->
+    h_tvarE_spec A (ReadTVar x) s a s
+| h_WriteTVar {A} (x : TVar A) (a b : A) s1 s2 :
+    s1 _ x = Some b ->
+    s2 _ x = Some a ->
+    (* s2 is the same as s1 except for x *) True ->
+    h_tvarE_spec unit (WriteTVar x a) s1 tt s2.
+
+Variant interp_state_specF {E F S} (h : forall A, E A -> S -> A -> S -> Prop) {A}
+  (sim : itree (E +' F) A -> S -> itree F (S * A) -> Prop):
+  itree' (E +' F) A -> S -> itree' F (S * A) -> Prop :=
+| InterpStateSpecRet a s : interp_state_specF h sim (RetF a) s (RetF (s, a))
+| InterpStateSpecTau t1 s t2 :
+    sim t1 s t2 ->
+    interp_state_specF h sim (TauF t1) s (TauF t2)
+| InterpStateSpecVis {X} (e : F X) k1 s k2 :
+    (forall x, sim (k1 x) s (k2 x)) ->
+    interp_state_specF h sim (VisF (inr1 e) k1) s (VisF e k2)
+| InterpStateSpecState {X} (e : E X) k1 s1 s2 r t2 :
+    h _ e s1 r s2 ->
+    sim (k1 r) s2 t2 ->
+    interp_state_specF h sim (VisF (inl1 e) k1) s1 (TauF t2).
+
+Definition interp_state_spec_ {E F S} h {A} sim (t1 : itree (E +' F) A) (s : S) t2 :=
+  interp_state_specF h sim (observe t1) s (observe t2).
+
+
+From Stdlib Require Import Basics.
+From Coinduction Require Import all.
+From Paco Require Import paco.
+From ITree Require Import Eq Eq.Shallow.
+
+Program Definition interp_state_specb {E F S} (h : forall A, E A -> S -> A -> S -> Prop) {A} :
+  mon (itree (E +' F) A -> S -> itree F (S * A) -> Prop) :=
+  {| body := interp_state_spec_ h |}.
+Next Obligation.
+  intros x y H t1 s t2 SR.
+  red in H.
+  red. red in SR.
+  genobs_clear t1 ot1.
+  genobs_clear t2 ot2.
+  inversion SR; subst.
+  - constructor.
+  - constructor. auto.
+  - constructor. auto.
+  - econstructor; eauto.
+Defined.
+
+
+
+Definition interp_state_spec {E F S} (h : forall A, E A -> S -> A -> S -> Prop) {A} :=
+  gfp (@interp_state_specb _ F _ h A).
+
+
+
+#[global] Instance interp_state_spec_cong_eqit_chain {E F S A} h (C : Chain (@interp_state_specb E F S h A)):
+  Proper (eq_itree eq ==> eq ==> eq_itree eq ==> flip impl) (elem C).
+Proof.
+  eapply (tower (P := fun R => Proper (eq_itree eq ==> eq ==> eq_itree eq ==> flip impl) R)).
+  { intros T HT t1 t1' EQ1 s s' Hs t2 t2' EQ2 H sim Tsim.
+    apply (HT sim Tsim t1 t1' EQ1 s s' Hs t2 t2' EQ2).
+    exact (H sim Tsim). }
+  clear C. intros C.
+  intros HC t1 t1' EQ1 s s' Hs t2 t2' EQ2 HI.
+  subst s'.
+  cbn in HI |- *. unfold interp_state_spec_ in HI |- *.
+  genobs t1' ot1'.
+  genobs t2' ot2'.
+  inversion HI; subst; clear HI.
+  - (* Ret *)
+    rewrite (simpobs H) in EQ1.
+    apply eqitree_inv_Ret_r in EQ1 as ->.
+    rewrite (simpobs H1) in EQ2.
+    apply eqitree_inv_Ret_r in EQ2 as ->.
+    constructor.
+  - (* Tau *)
+    rewrite (simpobs H0) in EQ1.
+    apply eqitree_inv_Tau_r in EQ1 as [? [-> ?]].
+    rewrite (simpobs H2) in EQ2.
+    apply eqitree_inv_Tau_r in EQ2 as [? [-> ?]].
+    constructor.
+    rewrite H1, H3.
+    assumption.
+  - (* Vis, right (non-handled) effect *)
+    rewrite (simpobs H0) in EQ1.
+    apply eqitree_inv_Vis_r in EQ1 as [? [-> ?]].
+    rewrite (simpobs H2) in EQ2.
+    apply eqitree_inv_Vis_r in EQ2 as [? [-> ?]].
+    constructor.
+    intros.
+    rewrite H1, H3.
+    apply H.
+  - (* Vis, left (handled/state) effect *)
+    rewrite (simpobs H1) in EQ1.
+    apply eqitree_inv_Vis_r in EQ1 as [? [-> ?]].
+    rewrite (simpobs H3) in EQ2.
+    apply eqitree_inv_Tau_r in EQ2 as [? [-> ?]].
+    econstructor; [eassumption|].
+    rewrite H2, H4.
+    assumption.
+Qed.
+
+#[global] Instance interp_state_spec_cong_eqit {E F S A} h :
+  Proper (eq_itree eq ==> eq ==> eq_itree eq ==> flip impl) (@interp_state_spec E F S h A).
+Proof.
+  unfold interp_state_spec.
+  apply gfp_prop, interp_state_spec_cong_eqit_chain.
+Qed.
